---
title: "Derivation of Bayes Theorem"
author: "Andy Grogan-Kaylor"
date: "`r Sys.Date()`"
output: 
  revealjs::revealjs_presentation:
    fig_height: 4
    highlight: haddock
    self_contained: no
    theme: default
    transition: convex
  html_document: 
    highlight: haddock
    theme: flatly
---

```{r setup, include=FALSE}

knitr::opts_chunk$set(echo = TRUE)

```

## Derivation

> Following inspiration from Kruschke (2011).

## From the definition of conditional probability: 

$P(A|B) = P(A,B) / P(B)$

$P(B|A) = P(A,B) / P(A)$

## Then: 

$P(A|B)P(B) = P(A,B)$

$P(B|A)P(A) = P(A,B)$

## Then:

$P(A|B)P(B) = P(B|A)P(A)$

## Then:

$P(A|B) = \frac{P(B|A)P(A)}{P(B)}$



