---
title: "Derivation of Bayes Theorem"
author: "Andy Grogan-Kaylor"
date: "today"
format: 
  html:
    css: styles.css
    toc: true
    number-sections: true
    theme:
      light: cosmo
      dark: vapor
---

# Derivation

> Following inspiration from Kruschke (2011).

# From The Definition Of Conditional Probability: 

$P(A|B) = P(A,B) / P(B)$

$P(B|A) = P(A,B) / P(A)$

# Multiply Each Fraction By The Denominator: 

$P(A|B)P(B) = P(A,B)$

$P(B|A)P(A) = P(A,B)$

# Set The Two Expressions To Be Equivalent:

$P(A|B)P(B) = P(B|A)P(A)$

# Divide by $P(B)$:

$P(A|B) = \frac{P(B|A)P(A)}{P(B)}$



